Remove BBStmt in AST.lean (#30)

MLIR/Dialects/ToySemantics.lean
@@ -35,12 +35,10 @@ inductive ToyOp: Type → Type :=
 /- To be automatically generated (hopefully; basically this is the
    verification stuff) -/
 
-def toy_semantics_op (ret_name: Option SSAVal) (op: Op builtin):
-      Fitree (UBE +' SSAEnvE builtin +' ToyOp) Unit :=
-
+def toy_semantics_op (op: Op builtin):
+    Fitree (UBE +' SSAEnvE builtin +' ToyOp) Unit :=
   match op with
-  | Op.mk "toy.constant" [] [] [] attrs
-        (.fn (.tuple []) (builtin.tensor D₁ τ₁)) =>
+  | Op.mk "toy.constant" [(res, builtin.tensor D₁ τ₁)] [] [] [] attrs =>
       match AttrDict.find attrs "value" with
       | some (builtin.dense_tensor_attr elem D₂ τ₂) =>
           match TensorLiteral.ofTensorElem elem D₁ τ₁ with
@@ -48,23 +46,23 @@ def toy_semantics_op (ret_name: Option SSAVal) (op: Op builtin):
               raiseUB s!"{op}"
           | some t_lit => do
               let t ← Fitree.trigger <| ToyOp.Constant D₁ τ₁ t_lit
-              SSAEnv.set? (builtin.tensor D₁ τ₁) ret_name t
+              SSAEnv.set? (builtin.tensor D₁ τ₁) res t
       | _ =>
           raiseUB s!"{op}"
 
-  | Op.mk "toy.transpose" [t_name] [] [] _ (.fn (builtin.tensor D τ) τ₂) =>
+  | Op.mk "toy.transpose" [(res, τ₂)] [(t_name, builtin.tensor D τ)] [] [] _ =>
       match D with
       | [Dimension.Known n, Dimension.Known m] => do
           let t ← Fitree.trigger (SSAEnvE.Get (builtin.tensor
                   [Dimension.Known n, Dimension.Known m] τ) t_name);
           let t' ← Fitree.trigger (ToyOp.Transpose τ n m t);
           SSAEnv.set? (builtin.tensor [Dimension.Known m, Dimension.Known n] τ)
-            ret_name t'
+            (some res) t'
       | _ =>
           raiseUB s!"{op}"
 
-  | Op.mk "toy.reshape" [t_name] [] [] _
-        (.fn (builtin.tensor D τ₁) (builtin.tensor D' τ₂)) =>
+  | Op.mk "toy.reshape" [(res, builtin.tensor D' τ₂)]
+        [(t_name, builtin.tensor D τ₁)] [] [] _ =>
       if H: τ₁ = τ₂
         ∧ DimList.known D
         ∧ DimList.known D'
@@ -73,18 +71,11 @@ def toy_semantics_op (ret_name: Option SSAVal) (op: Op builtin):
         let t' ← Fitree.trigger (ToyOp.Reshape τ₁ D D'
                 H.2.1 H.2.2.1 H.2.2.2 t);
         let t': RankedTensor D' τ₂ := cast (by rw [H.1]) t';
-        SSAEnv.set? (builtin.tensor D' τ₂) ret_name t'
+        SSAEnv.set? (builtin.tensor D' τ₂) (some res) t'
       else
         raiseUB s!"{op}"
 
   | _ => raiseUB s!"{op}"
-
-def toy_semantics_bbstmt: BasicBlockStmt builtin →
-      Fitree (UBE +' (SSAEnvE builtin) +' ToyOp) Unit
-  | BasicBlockStmt.StmtAssign val _ op =>
-      toy_semantics_op (some val) op
-  | BasicBlockStmt.StmtOp op =>
-      toy_semantics_op none op
 
 -- TODO: toy_semantics_bb: handle basic block arguments
 @[simp]
@@ -94,8 +85,8 @@ def toy_semantics_bb: BasicBlock builtin →
       Fitree.ret ()
   | BasicBlock.mk name args (op1::ops) =>
       List.foldr (fun t acc => Fitree.bind acc (fun _ => t))
-                 (toy_semantics_bbstmt op1)
-                 (ops.map toy_semantics_bbstmt)
+                 (toy_semantics_op op1)
+                 (ops.map toy_semantics_op)
 
 /- Manually specified: ToyOp event handler -/
 
@@ -123,24 +114,24 @@ def run_toy (t: Fitree (UBE +' SSAEnvE builtin +' ToyOp) Unit)
 -/
 
 -- TODO: Can we infer the builtin in there?
-def transpose_stmt: BasicBlockStmt builtin := [mlir_bb_stmt|
-  %t2 = "toy.transpose"(%t1): tensor<2×4×i32> -> tensor<4×2×i32>
+def transpose_stmt: Op builtin := [mlir_op|
+  %t2 = "toy.transpose"(%t1): (tensor<2×4×i32>) -> tensor<4×2×i32>
 ]
 
-def constant_stmt: BasicBlockStmt builtin := [mlir_bb_stmt|
+def constant_stmt: Op builtin := [mlir_op|
   %t = "toy.constant"() {value=dense<[[1,2],[3,4]]>: tensor<2×2×i32>}:
     () -> tensor<2×2×i32>
 ]
 
 def double_transpose: BasicBlock builtin := [mlir_bb|
   ^dbl:
-    %t2 = "toy.transpose"(%t1): tensor<2×4×i32> -> tensor<4×2×i32>
-    %t3 = "toy.transpose"(%t2): tensor<4×2×i32> -> tensor<2×4×i32>
+    %t2 = "toy.transpose"(%t1): (tensor<2×4×i32>) -> tensor<4×2×i32>
+    %t3 = "toy.transpose"(%t2): (tensor<4×2×i32>) -> tensor<2×4×i32>
 ]
 
-#eval Fitree.run <| run_toy (toy_semantics_bbstmt transpose_stmt) SSAEnv.empty
+#eval Fitree.run <| run_toy (toy_semantics_op transpose_stmt) SSAEnv.empty
 
-#eval Fitree.run <| run_toy (toy_semantics_bbstmt constant_stmt) SSAEnv.empty
+#eval Fitree.run <| run_toy (toy_semantics_op constant_stmt) SSAEnv.empty
 
 theorem double_transpose_correct:
   ∀ (t1: RankedTensor [.Known 2, .Known 4] .i32),
@@ -154,7 +145,7 @@ theorem double_transpose_correct:
       (SSAVal.SSAVal "t3", ⟨builtin.tensor [.Known 2, .Known 4] .i32, t1⟩)
     ]) := by
   intros t1
-  simp [double_transpose, toy_semantics_bb, toy_semantics_bbstmt]; simp_itree
+  simp [double_transpose, toy_semantics_bb, toy_semantics_op]; simp_itree
   simp [interpUB'!]; simp_itree
   simp [interpSSA', Fitree.interpState, SSAEnvE.handle]; simp_itree
   simp [SSAEnv.get, SSAEnv.set]; simp_itree
