MLIR/Semantics/Verifier.lean
@@ -38,36 +38,3 @@ instance {α} (o: Option α): Decidable (Option.isSome o) :=
   match o with
   | some value => isTrue rfl
   | none => isFalse (λ H => by simp [Option.isSome] at H)
-
-
-/- === Consistency between arity by argument count and operation type ===
-
-   Assuming custom syntax is expanded, the number of arguments and the
-   functional type of the operation must match. Equality can be structurally
-   enforced by weaving the lists together, morally changing
-
-     "op"(%arg, %arg, %arg): (!type, !type, !type) -> !ret
-
-   into the woven form
-
-     "op"(%arg:!type, %arg:!type, %arg!type): !ret
-
-   The number of arguments can also be specified at the same time. -/
-
-private def zip_args_types {α σ ε} {δ: Dialect α σ ε} (args: List SSAVal) (ty: MLIRType δ) :=
-  match args, ty with
-  | [], MLIRType.tuple [] =>
-      some []
-  | a::args, MLIRType.tuple (t::tys) =>
-      Option.map ((a,t) :: .) (zip_args_types args (MLIRType.tuple tys))
-  | [a], t =>
-      some [(a,t)]
-  | _, _ =>
-      none
-
--- This is the verifier function
-def vArgTypeArity: Verifier δ (List (SSAVal × MLIRType δ)) :=
-  fun (op: Op δ) =>
-    match op with
-    | Op.mk _ args _ _ _ (MLIRType.fn ty _) => zip_args_types args ty
-    | _ => none
